Remove admits in word_updN_shift proofs

src/Rec.v
@@ -769,64 +769,226 @@ Module Rec.
     exact (wlshift (combine (wones n) (wzero (n0 * n))) (idx * n)).
   Defined.
 
-
-  Theorem word_mask_gt : forall l n H idx, l > 0 ->
-    word_mask l n idx = eq_rec (n + (l * n - n)) word (combine (wones n) (wzero (l * n - n))) (l * n) H.
-  Proof.
-    intros l n.
-    remember (l * n - n) as e.
-    destruct l; auto.
-    intros; simpl in *.
-    assert (e = l * n) as HH by lia.
-    generalize dependent idx.
-    generalize dependent H.
-    generalize dependent H0.
-    rewrite HH.
-    intros.
-    eq_rect_simpl.
-    auto.
-  Qed.
-
-  Fact pow2_gt_0 : forall n, n > 0 -> n < pow2 n.
-  Proof.
-    induction n; try omega.
-    pose proof zero_lt_pow2 n.
-    simpl; omega.
-  Qed.
-
   Definition word_updN_shift (l n : nat) (idx : nat) (w : word (l * n))
                                              (v : word n) : word (l * n).
     destruct l eqn:H.
     exact w.
-    remember (zext v (n0 * n)) as v'.
-    remember (word_mask (S n0) n idx) as mask.
-    remember (n * idx) as shift.
-    remember (wlshift v' shift) as newmask.
+    set (v' := zext v (n0 * n)).
+    set (mask := word_mask (S n0) n idx).
+    set (shift := n * idx).
+    set (newmask := wlshift v' shift).
     exact ((w ^& (wnot mask)) ^| newmask).
   Defined.
 
-  Theorem word_mask_eq_combine_zero : forall n l idx H,
-    l > 0 -> idx < l ->
-    word_mask l n idx = split1 (l * n) n (
-    eq_rec (idx + (n + (l * n - idx))) word
-    (combine (wzero idx) (combine (wones n) (wzero (l * n - idx))))
-    (l * n + n) H).
+  Theorem word_updN_shift_l_gt_0 : forall idx off n H w v,
+    @word_updN_shift (idx + 1 + off) n idx w v = w ^& wnot (word_mask (idx + 1 + off) n idx) ^| wlshift (
+      eq_rect _ word (zext v ((idx + off) * n)) _ H) (idx * n).
+  Proof.
+    unfold word_updN_shift.
+    intros idx off.
+    replace (idx + 1 + off) with (S (idx + off)) by omega.
+    intros.
+    eq_rect_simpl.
+    f_equal.
+    f_equal.
+    apply mult_comm.
+  Qed.
+
+  Theorem word_mask_l_gt_0 : forall l n idx H, l > 0 ->
+    @word_mask l n idx = wlshift (
+      eq_rect _ word (combine (wones n) (wzero ((l - 1) * n))) _ H)
+      (idx * n).
+  Proof.
+    unfold word_mask; destruct l; auto; intros.
+    erewrite combine_eq_rect2.
+    repeat f_equal.
+    generalize_proof.
+    intros HH; rewrite HH; auto.
+    Grab Existential Variables. lia.
+  Qed.
+
+  Theorem eq_rect_combine_dist3 : forall a b c H H1 H2 (w : word ((a + 1 + b) * c)),
+    let w' := eq_rect ((a + 1 + b) * c) word w _ H1 in
+    let w'' := eq_rect ((a + 1 + b) * c) word w _ H2 in
+    w = eq_rect _ word (combine
+      (split1 (a * c) _ w')
+      (combine
+        (middle (a * c) c (b * c) w')
+        (split2 (a * c + c) (b * c) w''))) _ H.
+  Proof.
+    intros a b c H.
+    rewrite <- H.
+    intros.
+    subst w' w''.
+    eq_rect_simpl.
+    unfold middle.
+    rewrite <- combine_split with (w := w).
+    repeat f_equal; rewrite combine_split; auto.
+    erewrite <- eq_rect_word_match.
+    rewrite combine_end.
+    reflexivity.
+  Qed.
+
+  Fact split1_eq_rect_combine_partial_helper : forall a b c d (H : a + c = a + b + d), c = b + d.
+  Proof. intros. omega. Qed.
+
+  Theorem split1_eq_rect_combine_partial : forall a b c d H (wa : word a) (wc : word c),
+    split1 (a + b) d
+      (eq_rect (a + c) word (combine wa wc) (a + b + d) H) =
+        combine wa (split1 b d (eq_rect _ word wc _ (split1_eq_rect_combine_partial_helper a b c d H))).
+  Proof.
+    intros a b c d H.
+    assert (c = b + d) by omega; subst c.
+    intros.
+    erewrite <- split1_combine; f_equal.
+    eq_rect_simpl.
+    erewrite combine_assoc.
+    rewrite eq_rect_word_match.
+    rewrite combine_split.
+    reflexivity.
+  Qed.
+
+  Theorem wnot_word_mask_l_gt_0 : forall off n idx H,
+    wnot (@word_mask (idx + 1 + off) n idx) = eq_rec _ word (
+    combine (wones (idx * n)) (combine (wzero n) (wones (off * n)))) ((idx + 1 + off) * n) H.
+  Proof.
+    intros off n idx.
+    replace (idx + 1 + off) with (S (idx + off)) by omega.
+    intros.
+    unfold word_mask.
+    rewrite wnot_wlshift.
+    eq_rect_simpl.
+    erewrite split1_eq_rect_eq1; f_equal.
+    eq_rect_simpl.
+    rewrite split1_eq_rect_combine_partial; f_equal.
+    rewrite wnot_combine, wnot_ones.
+    rewrite split1_eq_rect_combine_partial; f_equal.
+    erewrite wzero_dist, wzero_rev, <- combine_wzero.
+    repeat rewrite wnot_eq_rect.
+    eq_rect_simpl.
+    rewrite wnot_combine, split1_combine.
+    apply wnot_zero.
+    Grab Existential Variables.
+    all : lia.
+  Qed.
+
+  Lemma wand_wnot_word_mask_w : forall idx off n H1 H2 H3 w,
+    let w' := eq_rect _ word w (idx * n + (n + off * n)) H1 in
+    let w'' := eq_rect _ word w (idx * n + n + off * n) H2 in
+    w ^& wnot (word_mask (idx + 1 + off) n idx) = eq_rec _ word (
+      combine (split1 (idx * n) _ w') (combine (wzero n) (split2 (idx * n + n) _ w''))) _ H3.
   Proof.
     intros.
-    assert (l * n >= n) by (induction l; lia).
-    erewrite word_mask_gt; auto.
-  Admitted.
+    erewrite eq_rect_combine_dist3 with (w := w).
+    erewrite wnot_word_mask_l_gt_0 by omega.
+    unfold wand.
+    unfold eq_rec.
+    erewrite <- eq_rect_bitwp'; f_equal.
+    repeat erewrite <- combine_bitwp; f_equal.
+    - rewrite wand_comm, wand_wones.
+      reflexivity.
+    - rewrite wand_comm, wand_wzero.
+      rewrite wand_comm, wand_wones.
+      reflexivity.
+  Qed.
+
+  Fact eq_rect_combine_assoc' : forall a b c H wa wb wc,
+    eq_rect (a + (b + c)) word (combine wa (combine wb wc)) _ H = combine (combine wa wb) wc.
+  Proof.
+    intros.
+    erewrite combine_assoc, eq_rect_word_match.
+    reflexivity.
+  Qed.
+
+  Theorem word_updN_shift_abs : forall off idx n H1 H2 H3 w v,
+    let w' := eq_rec _ word w _ H1 in
+    let w'' := eq_rec _ word w _ H2 in
+    @word_updN_shift (idx + 1 + off) n idx w v = eq_rec _ word (
+      combine (split1 (idx * n) (n + off * n) w')
+      (combine v (split2 (idx * n + n) (off * n) w''))) _ H3.
+  Proof.
+    intros.
+    assert ((idx + 1 + off) * n = idx * n + n + off * n) as Hc by lia.
+    erewrite eq_rect_combine_dist3 with (w := w).
+    erewrite word_updN_shift_l_gt_0.
+    erewrite wand_wnot_word_mask_w.
+    unfold wlshift, zext.
+    eq_rect_simpl.
+    rewrite split1_combine.
+    rewrite eq_rect_combine_assoc'.
+    rewrite split2_combine.
+    unfold wor.
+    rewrite eq_rect_bitwp_1.
+    f_equal.
+    replace (eq_rect ((idx + 1 + off) *n) word (split1 _ (idx * n) _) _ _)
+      with (combine (wzero (idx * n)) (combine v (wzero (off * n)))).
+    - repeat rewrite <- combine_bitwp.
+      repeat rewrite wor_wzero.
+      repeat try (rewrite wor_comm, wor_wzero).
+      reflexivity.
+    - erewrite split1_eq_rect_eq1.
+      repeat (eq_rect_simpl; erewrite split1_eq_rect_combine_partial; f_equal).
+      erewrite wzero_dist, wzero_rev, <- combine_wzero.
+      eq_rect_simpl.
+      symmetry; apply split1_combine.
+    Grab Existential Variables.
+    all : lia.
+  Qed.
+
+  Fact word_updN_abs_helper : forall idx off, idx < idx + 1 + off.
+  Proof. intros. omega. Qed.
+
+  Fact eq_rect_both_helper : forall T (x y z : T), x = y -> z = y -> z = x.
+  Proof. intros. subst. reflexivity. Qed.
+
+  Theorem eq_rect_both : forall x y z (H1 : x = z) (H2 : y = z) wa wb,
+    wa = eq_rect y word wb x (eq_rect_both_helper H1 H2) -> eq_rect x word wa z H1 = eq_rect y word wb z H2.
+  Proof.
+    intros. subst.
+    eq_rect_simpl.
+    reflexivity.
+   Qed.
+
+  Theorem word_updN_abs : forall idx off ft H H1 H2 w v,
+    let w' := eq_rec _ word w _ H1 in
+    let w'' := eq_rec _ word w _ H2 in
+    @word_updN ft (idx + 1 + off) idx w v = eq_rec _ word (
+      combine (split1 (idx * len ft) (len ft + off * len ft) w')
+        (combine v (split2 (idx * len ft + len ft) (off * len ft) w''))) _ H.
+  Proof.
+    unfold word_updN; simpl.
+    intros.
+    destruct lt_dec; try omega.
+    repeat eexists.
+    eq_rect_simpl; apply eq_rect_both.
+    rewrite eq_rect_word_offset; eq_rect_simpl.
+    rewrite eq_rect_combine; f_equal.
+    + erewrite eq_rect_split1_eq2.
+      eq_rect_simpl; f_equal.
+      apply eq_rect_both.
+      eq_rect_simpl; reflexivity.
+    + apply eq_rect_both.
+      rewrite eq_rect_combine.
+      rewrite eq_rect_split2.
+      eq_rect_simpl.
+      repeat (try reflexivity; f_equal; eq_rect_simpl; try apply eq_rect_both).
+    Grab Existential Variables.
+    all : simpl; lia.
+  Qed.
 
   Theorem word_updN_shift_equiv : forall l idx ft w v, idx < l ->
     @word_updN_shift l (len ft) idx w v = @word_updN ft l idx w v.
   Proof.
-    destruct l; auto.
-    intros.
-    unfold word_updN_shift.
-    erewrite word_mask_eq_combine_zero by omega.
-    unfold word_updN.
-    destruct lt_dec; try omega.
-  Admitted.
+    intros l idx ft w v H.
+    remember (l - idx - 1) as off.
+    assert (l = idx + 1 + off) by omega.
+    subst l.
+    erewrite word_updN_shift_abs by auto.
+    erewrite word_updN_abs.
+    repeat f_equal.
+    Grab Existential Variables.
+    all : lia.
+  Qed.
 
   Definition word_updN' {ft : type} {l : nat} (idx : nat) (w : word (len (ArrayF ft l)))
             (v : word (len ft)) : word (len (ArrayF ft l)) := @word_updN_shift l (len ft) idx w v.
